theories/ConfigUtils.v
@@ -13,6 +13,7 @@ From Peregrine Require Import OCamlBackend.
 From Peregrine Require Import CakeMLBackend.
 From Peregrine Require Import CBackend.
 From Peregrine Require Import WasmBackend.
+From Peregrine Require Import EvalBackend.
 
 Local Open Scope bs_scope.
 
@@ -170,13 +171,32 @@ Section BackendConfigOptional.
 
   Definition mk_cakeml_config (o : cakeml_config') : cakeml_config := tt.
 
+  Record eval_config' := {
+    copts'    : option certicoq_config';
+    fuel'     : nat;
+    eval_anf' : bool;
+  }.
+  Definition empty_eval_config' : eval_config' := {|
+    copts'    := None;
+    fuel'     := (Nat.pow 2 14);
+    eval_anf' := true;
+  |}.
+
+  Definition mk_eval_config (o : eval_config') : eval_config := {|
+    copts    := get_optional o default_eval_config
+      (fun c => option_map (mk_certicoq_config default_eval_config.(copts)) (copts' c)) copts;
+    fuel     := o.(fuel');
+    eval_anf := o.(eval_anf');
+  |}.
+
   Inductive backend_config' :=
   | Rust'   : rust_config' -> backend_config'
   | Elm'    : elm_config' -> backend_config'
   | C'      : c_config' -> backend_config'
   | Wasm'   : wasm_config' -> backend_config'
   | OCaml'  : ocaml_config' -> backend_config'
-  | CakeML' : cakeml_config' -> backend_config'.
+  | CakeML' : cakeml_config' -> backend_config'
+  | Eval'   : eval_config' -> backend_config'.
   Definition mk_backend_config (o : backend_config') : backend_config :=
     match o with
     | Rust' o   => Rust (mk_rust_config o)
@@ -185,6 +205,7 @@ Section BackendConfigOptional.
     | Wasm' o   => Wasm (mk_certicoq_config default_wasm_config o)
     | OCaml' o  => OCaml (mk_ocaml_config o)
     | CakeML' o => CakeML (mk_cakeml_config o)
+    | Eval' o => Eval (mk_eval_config o)
     end.
 
 End BackendConfigOptional.
@@ -259,6 +280,7 @@ Section GeneralConfigOptional.
       | Wasm' _   => get_default_phases_opt wasm_phases
       | OCaml' _  => get_default_phases_opt ocaml_phases
       | CakeML' _ => get_default_phases_opt cakeml_phases
+      | Eval' _   => get_default_phases_opt eval_phases
       end in
     match o with
     | Some o =>
@@ -269,6 +291,7 @@ Section GeneralConfigOptional.
       | Wasm' _   => enforce_phases o def_opt wasm_phases
       | OCaml' _  => enforce_phases o def_opt ocaml_phases
       | CakeML' _ => enforce_phases o def_opt cakeml_phases
+      | Eval' _   => enforce_phases o def_opt eval_phases
       end
     | None => def_opt
     end.
@@ -361,6 +384,12 @@ Section GeneralConfigOptional.
   Definition is_wasm_config (o : config) : bool :=
     match o.(backend_opts) with
     | Wasm _ => true
+    | _ => false
+    end.
+
+  Definition is_eval_config (o : config) : bool :=
+    match o.(backend_opts) with
+    | Eval _ => true
     | _ => false
     end.
 
