theories/backends/EvalBackend.v
@@ -1,0 +1,75 @@
+From MetaRocq.Utils Require Import utils.
+From MetaRocq.Utils Require Import bytestring.
+From MetaRocq.Erasure.Typed Require Import ResultMonad.
+From CertiCoq Require Import Compiler.pipeline.
+From CertiCoq Require Import Common.Pipeline_utils.
+From Peregrine Require Import Config.
+From Peregrine Require Import Utils.
+From Peregrine Require Import CertiCoqBackend.
+From Peregrine Require Import EvalBox.
+From ExtLib.Structures Require Import Monad.
+
+Import MonadNotation.
+
+Local Open Scope bs_scope.
+
+
+
+Definition default_eval_config := {|
+  copts           := {|
+    direct    := true;
+    c_args    := 5;
+    o_level   := 0;
+    anf_conf  := 0;
+    prefix    := "";
+    body_name := "body";
+  |};
+  Config.fuel     := (Nat.pow 2 14);
+  Config.eval_anf := true;
+|}.
+
+Definition eval_phases := {|
+  implement_box_c  := Required;
+  implement_lazy_c := Compatible false;
+  cofix_to_laxy_c  := Compatible false;
+  betared_c        := Compatible false;
+  unboxing_c       := Compatible false;
+  dearg_ctors_c    := Compatible false;
+  dearg_consts_c   := Compatible false;
+|}.
+
+
+
+Definition eval_anf_pipeline prs fuel (p : EAst.program) :=
+  let env := p.1 in
+  '(prs, next_id) <- register_prims prs next_id env ;;
+  p_anf <- anf_pipeline p prs next_id;;
+  (* Eval using ANF evaluator *)
+  p_v <- eval_anf fuel p_anf;;
+  ret p_v.
+
+Definition eval_mut_pipeline prs fuel (p : EAst.program) :=
+  let env := p.1 in
+  '(prs, next_id) <- register_prims prs next_id env ;;
+  p_anf <- mut_pipeline p prs;;
+  (* Eval using mut evaluator *)
+  p_v <- eval_mut fuel p_anf;;
+  ret p_v.
+
+
+
+Definition eval (remaps : constant_remappings)
+                (custom_attr : custom_attributes)
+                (opts : eval_config)
+                (file_name : string)
+                (p : EAst.program)
+                : result string string :=
+  let config := mk_opts opts.(Config.copts) in
+  let prs := mk_prims remaps in
+  let evaluator := if opts.(Config.eval_anf) then eval_anf_pipeline else eval_mut_pipeline in
+  let (res, _) :=
+    run_pipeline EAst.program string config p (evaluator prs opts.(Config.fuel)) in
+  match res with
+  | compM.Ret s => Ok s
+  | compM.Err s => Err s
+  end.
