theories/serialization/SerializeConfigSound.v
@@ -210,12 +210,51 @@ Proof.
   exact He.
 Qed.
 
+Instance Sound_eval_config : SoundClass eval_config.
+Proof.
+  unfold SoundClass, Sound.
+  intros l e a He.
+  apply sound_match_con in He.
+  destruct He as [He | He]; elim_Exists He.
+  destruct He as [es [<- He]].
+  sound_field He.
+  apply sound_class in Ea0.
+  apply sound_class in Ea1.
+  apply sound_class in Ea2.
+  unfold to_sexp, Serialize_eval_config.
+  cbn.
+  rewrite <- Ea0, <- Ea1, <- Ea2.
+  reflexivity.
+Qed.
+
+Instance Sound_eval_config' : SoundClass eval_config'.
+Proof.
+  unfold SoundClass, Sound.
+  intros l e a He.
+  apply sound_match_con in He.
+  destruct He as [He | He]; elim_Exists He.
+  destruct He as [es [<- He]].
+  sound_field He.
+  apply sound_class in Ea0.
+  apply sound_class in Ea1.
+  apply sound_class in Ea2.
+  unfold to_sexp, Serialize_eval_config'.
+  cbn.
+  rewrite <- Ea0, <- Ea1, <- Ea2.
+  reflexivity.
+Qed.
+
 Instance Sound_backend_config : SoundClass backend_config.
 Proof.
   unfold SoundClass, Sound.
   intros l e n He.
   apply sound_match_con in He.
   destruct He as [He | He]; elim_Exists He.
+  - destruct He as [es [<- He]].
+    sound_field He.
+    apply sound_class in Ea1.
+    rewrite <- Ea1.
+    reflexivity.
   - destruct He as [es [<- He]].
     sound_field He.
     apply sound_class in Ea1.
@@ -254,6 +293,11 @@ Proof.
   intros l e n He.
   apply sound_match_con in He.
   destruct He as [He | He]; elim_Exists He.
+  - destruct He as [es [<- He]].
+    sound_field He.
+    apply sound_class in Ea1.
+    rewrite <- Ea1.
+    reflexivity.
   - destruct He as [es [<- He]].
     sound_field He.
     apply sound_class in Ea1.
